Defined new "weak" version of frame preservation

ulib/FStar.PCM.fst
@@ -124,6 +124,44 @@ let compatible_elim
     goal #a #(fun frame -> composable pcm x frame /\ op pcm frame x == y)
     () (fun frame -> lemma frame)
 
+let compatible_intro
+  (#a: Type u#a) (pcm:pcm a) (x y:a)
+  (frame: a)
+  : Lemma
+    (requires (composable pcm x frame /\ op pcm frame x == y))
+    (ensures (compatible pcm x y))
+  = ()
+
+let frame_preserving_weak (#a: Type u#a) (pcm:pcm a) (x y: a) : prop =
+    (forall frame. composable pcm frame x ==> composable pcm frame y) /\
+    (forall frame.{:pattern (composable pcm frame x)} composable pcm frame x ==> compatible pcm frame y)
+
+let frame_preserving_weak_intro (#a: Type u#a) (pcm:pcm a) (x y: a)
+  (lemma1: (frame: a) -> Lemma (requires composable pcm frame x) (ensures composable pcm frame y))
+  (lemma2: (frame: a) -> Lemma
+    (requires composable pcm frame x /\ composable pcm frame y)
+    (ensures compatible pcm frame y)
+  )
+  : Lemma (frame_preserving_weak pcm x y)
+  =
+  let aux1 (frame: a) : Lemma (composable pcm frame x ==> composable pcm frame y) =
+    let aux2 (_: squash (composable pcm frame x)) : Lemma (composable pcm frame y) =
+      lemma1 frame
+    in
+    Classical.impl_intro aux2
+  in
+  Classical.forall_intro aux1;
+  let aux3 (frame: a): Lemma (composable pcm frame x ==> compatible pcm frame y) =
+    let aux4 (_: squash (composable pcm frame x)) : Lemma (
+      composable pcm frame x /\ (aux1 frame; compatible pcm frame y)
+    ) =
+      lemma2 frame
+    in
+    Classical.impl_intro aux4
+  in
+
+  Classical.forall_intro aux3
+
 (**
   To understand this predicate, one must consider the context of mutating the element [x] to
   element [y] under the rules of [pcm]. This mutation operation is frame-preserving if:
@@ -158,6 +196,43 @@ let frame_preserving_intro (#a: Type u#a) (pcm:pcm a) (x y: a)
     Classical.impl_intro aux4
   in
   Classical.forall_intro aux3
+
+let frame_preserving_implies_weak
+  (#a: Type u#a)
+  (pcm:pcm a)
+  (x y: a)
+  : Lemma (frame_preserving pcm x y ==> frame_preserving_weak pcm x y)
+  =
+  let aux (_ : squash (frame_preserving pcm x y)) : Lemma (frame_preserving_weak pcm x y) =
+    frame_preserving_weak_intro pcm x y
+      (fun frame -> ())
+      (fun frame ->
+        pcm.comm y frame;
+        compatible_intro pcm frame y y
+      )
+  in
+  Classical.impl_intro aux
+
+let frame_preserving_weak_with_full_update
+  (#a: Type u#a)
+  (pcm:pcm a)
+  (x y: a)
+  (full_update: (frame: a) -> Lemma
+    (requires (composable pcm x frame))
+    (ensures (frame == pcm.p.one))
+  )
+  : Lemma (frame_preserving_weak pcm x y ==> frame_preserving pcm x y)
+  =
+  let aux (_: squash (frame_preserving_weak pcm x y)) : Lemma (frame_preserving pcm x y) =
+    frame_preserving_intro pcm x y
+      (fun frame -> ())
+      (fun frame ->
+       full_update frame;
+       pcm.comm y frame;
+       pcm.is_unit y
+      )
+  in
+  Classical.impl_intro aux
 
 (** The PCM [p] is exclusive to element [x] if the only element composable with [x] is [p.one] *)
 let exclusive (#a:Type u#a) (p:pcm a) (x:a) =
